

**Problem §2.3: 2:** Determine whether  $f$  is a function from  $\mathbb{Z}$  to  $\mathbb{R}$  if

- (a)  $f(n) = \pm n$
- (b)  $f(n) = \sqrt{n^2 + 1}$
- (c)  $f(n) = \frac{1}{n^2 - 4}$

*Solution.* (a) **No.** This is not a function because  $f(n)$  is not well-defined, i.e. it does not map each element of the domain to a *single* element of the codomain.

(b) **Yes.** For all  $z \in \mathbb{Z}$ , the image  $f(z) = \sqrt{z^2 + 1}$  is well-defined and lies in the codomain,  $\mathbb{R}$ .

(c) **No**, because  $f(z)$  is not defined for all  $z \in \mathbb{Z}$ . Observe that for both  $z = 2$  and  $z = -2$ ,  $f(z)$  is undefined because it would involve division by zero. In order for  $f(n)$  to be a function with domain  $\mathbb{Z}$ , it would need to be defined on all elements of  $\mathbb{Z}$ . □

**Problem §2.3: 12:** Determine whether each of these functions from  $\mathbb{Z}$  to  $\mathbb{Z}$  is one-to-one.

- (a)  $f(n) = n - 1$ .
- (b)  $f(n) = n^2 + 1$ .
- (c)  $f(n) = n^3$ .
- (d)  $f(n) = \lceil n/2 \rceil$ .

*Solution.* Recall that a function  $f : A \rightarrow B$  is one-to-one if  $f(a_1) = f(a_2)$  implies  $a_1 = a_2$  for all  $a_1, a_2 \in A$ . To show that a function is not one-to-one, it is sufficient to find a single counterexample where  $a_1 \neq a_2$  but  $f(a_1) = f(a_2)$  for some  $a_1, a_2 \in A$ .

**Yes**, this function is one-to-one. For any  $n_1, n_2 \in \mathbb{Z}$ , observe that if  $f(n_1) = f(n_2)$  then

$$f(n_1) = n_1 - 1 = n_2 - 1 = f(n_2),$$

which implies that  $n_1 = n_2$ .

(b) **No**, this function is not one-to-one. Observe that, for example,

$$f(-2) = (-2)^2 + 1 = 5 = 2^2 + 1 = f(2),$$

but  $-2 \neq 2$ .

(c) **Yes**, this function is one-to-one. For any  $n_1, n_2 \in \mathbb{Z}$ , observe that if  $f(n_1) = f(n_2)$  then

$$f(n_1) = n_1^3 = n_2^3 = f(n_2),$$

which implies that  $n_1 = n_2$  because all real numbers have a unique cube root.

(d) **No**, this function is not one-to-one. For example, observe that

$$f(3) = \lceil 3/2 \rceil = 2 = \lceil 4/2 \rceil = f(4),$$

but  $3 \neq 4$ . □

**Problem §2.3: 14(a,b,c,d):** Determine whether  $f : \mathbb{Z} \times \mathbb{Z} \rightarrow \mathbb{Z}$  is onto if

- (a)  $f(m, n) = 2m - n$ .
- (b)  $f(m, n) = m^2 - n^2$ .
- (c)  $f(m, n) = m + n + 1$ .
- (d)  $f(m, n) = |m| - |n|$ .

*Solution.* Recall that a function  $f : A \rightarrow B$  is onto if for every  $b \in B$ , there exists some  $a \in A$  such that  $f(a) = b$ . To show that a function is not onto, it's sufficient to find a single  $b \in B$  that is not the image of any element of the domain,  $A$ .

- (a) **Yes**, this function is onto. Observe that any integer  $z$  in the codomain,  $\mathbb{Z}$ , is the image of  $(0, -z)$ :

$$f(0, -z) = 2(0) - (-z) = z.$$

- (b) **No**, this function is not onto. For example, 2 is in its codomain but not its range. Observe that if

$$m^2 - n^2 = (m - n)(m + n) = 2,$$

then  $m$  and  $n$  must have the same parity, i.e. must both either be even or odd (if  $m$  and  $n$  had different parities, then both  $m - n$  and  $m + n$  would be odd, forcing their product,  $m^2 - n^2$ , to also be odd). If  $m$  and  $n$  have the same parity, then both  $m - n$  and  $m + n$  are even and therefore divisible by 2. Hence, their product is divisible by 4 and cannot be equal to 2.

- (c) **Yes**, this function is onto. Observe that any integer  $z$  in the codomain  $\mathbb{Z}$  is the image of  $(0, z - 1)$ :

$$f(0, z - 1) = 0 + (z - 1) + 1 = z.$$

- (d) **Yes**, this function is onto. Observe that any positive integer  $z$  in the codomain  $\mathbb{Z}$  is the image of  $(z, 0)$ , any negative integer  $z$  is the image of  $(0, z)$ , and 0 is the image of  $(0, 0)$ :

$$\begin{aligned} f(z, 0) &= |z| - |0| = |z| = z, & \text{for } z \in \mathbb{Z}_{\geq 0}, \\ f(0, z) &= |0| - |z| = -|z| = -(-z) = z, & \text{for } z \in \mathbb{Z}_{\leq 0}, \\ f(0, 0) &= |0| - |0| = 0. \end{aligned}$$

□

**Problem §2.3: 20:** Give an example of a function from  $\mathbb{N}$  to  $\mathbb{N}$  that is

- (a) one-to-one but not onto.
- (b) onto but not one-to-one.
- (c) both onto and one-to-one (but not the identity function).
- (d) neither one-to-one nor onto.

*Solution.* (a) The function  $f(n) = n + 1$  is one-to-one but not onto. To see that it's one-to-one, observe that for all  $n_1, n_2 \in \mathbb{N}$ , if  $f(n_1) = f(n_2)$  then  $n_1 + 1 = n_2 + 1$  which implies  $n_1 = n_2$ . It's not onto, however, because 0 is not the image of any natural number. To see this, observe that if we had  $0 = f(n) = n + 1$ , this would require that  $n = -1$  and  $-1 \notin \mathbb{N}$ .

- (b) The function  $f(n) = \lceil n/2 \rceil$  is onto but not one-to-one. Observe that any element  $n$  of the codomain is the image of both  $2n$  and  $2n + 1$ :

$$\begin{aligned} f(2n) &= \lceil (2n)/2 \rceil = \lceil n \rceil = n, \\ f(2n + 1) &= \lceil \frac{2n + 1}{2} \rceil = \lceil n + 1/2 \rceil = n. \end{aligned}$$

(c) Consider the piecewise function

$$f(n) = \begin{cases} n-1 & n \text{ even} \\ n+1 & n \text{ odd} \end{cases}$$

which “swaps” the even and odd natural numbers. For example,  $f(1) = 2$  and  $f(2) = 1$ ,  $f(3) = 4$  and  $f(4) = 3$ , etc. This function is onto because each even  $n$  in the codomain is the image of  $n-1$  and each odd  $n$  in the codomain is the image of  $n+1$ . It is also one-to-one. To see that it is one-to-one, observe that if  $f(n_1) = f(n_2)$ , then either  $n_1 - 1 = n_2 - 1$  or  $n_1 + 1 = n_2 + 1$ , depending on parity. In either case, this implies  $n_1 = n_2$ .

(d) The function  $f(n) = 0$  is clearly neither onto nor one-to-one because it maps every element of the domain to the same element of the codomain.

□

**Problem §2.3: 22(a,b):** Determine whether each of these functions is a bijection from  $\mathbb{R}$  to  $\mathbb{R}$ .

(a)  $f(x) = -3x + 4$ .

(b)  $f(x) = -3x^2 + 7$ .

*Solution.* Recall that a bijection is a function that is both injective (one-to-one) and surjective (onto). So one strategy would be to determine if each function is both injective or surjective. To save ourselves some work, though, when we want to show that a function is a bijection we can use the fact that only bijections have inverses. Showing that an inverse function exists is, therefore, equivalent to showing that the function is a bijection.

(a) **Yes**, this function is a bijection. We claim that the inverse function of  $f$  is  $f^{-1}(x) = (4-x)/3$ . To verify this, observe that for  $x \in \mathbb{R}$ ,

$$\begin{aligned} (f^{-1} \circ f)(x) &= f^{-1}(f(x)) = f^{-1}(-3x + 4) = \frac{4 - (-3x + 4)}{3} = \frac{3x}{3} = x, \\ (f \circ f^{-1})(x) &= f(f^{-1}(x)) = f\left(\frac{4-x}{3}\right) = -3\left(\frac{4-x}{3}\right) + 4 = -4 + x + 4 = x \end{aligned}$$

(b) **No**, this function is not a bijection because it's not injective *or* surjective. To see that it's not injective, observe that, for example,  $f(-1) = -3(-1)^2 + 7 = 4 = -3(1)^2 + 7 = f(1)$ , but  $-1 \neq 1$ . To see that it's not surjective, observe that  $x^2 \geq 0$  for all  $x \in \mathbb{R}$ . As such, the range of  $f(x)$  is  $(-\infty, 7]$ , which is clearly not equal to the codomain  $\mathbb{R}$ .

□

**Problem §2.3: 36:** Find  $f \circ g$  and  $g \circ f$  where  $f(x) = x^2 + 1$  and  $g(x) = x + 2$  are functions from  $\mathbb{R}$  to  $\mathbb{R}$ .

*Solution.* Because both  $f$  and  $g$  are functions from  $\mathbb{R}$  to  $\mathbb{R}$ , the compositions  $f \circ g$  and  $g \circ f$  are well-defined. We can compute these compositions as:

$$\begin{aligned} (f \circ g)(x) &= f(g(x)) = f(x + 2) = (x + 2)^2 + 1 = x^2 + 4x + 5, \\ (g \circ f)(x) &= g(f(x)) = g(x^2 + 1) = x^2 + 1 + 2 = x^2 + 3. \end{aligned}$$

Notice that  $g \circ f \neq f \circ g$ !

□

**Problem §2.3: 39:** Show that the function  $f(x) = ax + b$  from  $\mathbb{R}$  to  $\mathbb{R}$  is invertible, where  $a$  and  $b$  are constants, with  $a \neq 0$ , and find the inverse of  $f$ .

*Solution.* One easy way to show that the given function  $f$  is invertible is to exhibit an inverse function. We claim that it has inverse function

$$f^{-1} : \mathbb{R} \rightarrow \mathbb{R}$$

$$x \mapsto \frac{x - b}{a}.$$

To verify that this is the inverse function of  $f$ , we need to check that both  $(f \circ f^{-1})$  and  $(f^{-1} \circ f)$  are the identity function on  $\mathbb{R}$ . We can do so by computing

$$(f \circ f^{-1})(x) = f(f^{-1}(x)) = f\left(\frac{x - b}{a}\right) = a\left(\frac{x - b}{a}\right) + b = x - b + b = x,$$

$$(f^{-1} \circ f)(x) = f^{-1}(f(x)) = f^{-1}(ax + b) = \frac{(ax + b) - b}{a} = \frac{ax}{a} = x.$$

□

**Problem §2.3: 40(a):** Let  $f$  be a function from the set  $A$  to the set  $B$ . Let  $S$  and  $T$  be subsets of  $A$ . Show that  $f(S \cup T) = f(S) \cup f(T)$ .

*Solution.* We'll show that  $f(S \cup T) = f(S) \cup f(T)$  by showing that each set is a subset of the other.

First, suppose that  $b \in f(S \cup T)$ . By definition, this means that  $b = f(a)$  for some  $a \in S \cup T$ . By definition of union, either  $a \in S$ ,  $a \in T$ , or both. If  $a \in S$ , then  $f(a) \in f(S)$ . If  $a \in T$ , then  $f(a) \in f(T)$ . Thus, in any case we have  $f(a) \in f(S) \cup f(T)$ . Hence,  $f(S \cup T) \subseteq f(S) \cup f(T)$ .

Conversely, suppose that  $b \in f(S) \cup f(T)$ . Then by definition,  $b \in f(S)$  or  $b \in f(T)$  or both. If  $b \in f(S)$ , then by definition  $b = f(a)$  for some  $a \in S$ . Similarly, if  $b \in f(T)$  then by definition  $b = f(a)$  for some  $a \in T$ . So in every case, we have  $b = f(a)$  for some  $a \in S \cup T$  and by definition  $b \in f(S \cup T)$ .

Since we've shown both inclusions, we have therefore shown that  $f(S \cup T) = f(S) \cup f(T)$ , as desired. □

**Problem §2.3: 44(b):** Let  $f$  be a function from  $A$  to  $B$ . Let  $S$  and  $T$  be subsets of  $B$ . Show that  $f^{-1}(S \cap T) = f^{-1}(S) \cap f^{-1}(T)$ .

*Solution.* Again, we'll show the desired set equality by showing that each set is a subset of the other.

First, consider  $a \in f^{-1}(S \cap T)$ . By definition,  $f(a) \in S \cap T$  and therefore either  $f(a) \in S$  and  $f(a) \in T$ . The fact that  $f(a) \in S$  means  $a \in f^{-1}(S)$ . Similarly, the fact that  $f(a) \in T$  means that  $a \in f^{-1}(T)$ . Hence, by definition  $a \in f^{-1}(S) \cap f^{-1}(T)$  and  $f^{-1}(S \cap T) \subseteq f^{-1}(S) \cap f^{-1}(T)$ .

Conversely, consider  $a \in f^{-1}(S) \cap f^{-1}(T)$ . By definition,  $a \in f^{-1}(S)$  and  $a \in f^{-1}(T)$ . From the definition of the preimage of a set, we know that  $a \in f^{-1}(S)$  means that  $f(a) \in S$ . Similarly,  $a \in f^{-1}(T)$  means that  $f(a) \in T$ . As such, we have  $f(a) \in S \cap T$  and therefore  $a \in f^{-1}(S \cap T)$ . Thus,  $f^{-1}(S) \cap f^{-1}(T) \subseteq f^{-1}(S \cap T)$ .

Because we've shown both inclusions, we have therefore shown that  $f^{-1}(S \cap T) = f^{-1}(S) \cap f^{-1}(T)$ , as desired. □